src/program_proof/txn/twophase_refinement_proof.v
@@ -39,7 +39,7 @@ Proof.
   rewrite /sty_init_obligation1//=.
   iIntros (? hG hRG hJrnl σs gs σi gi Hinit) "Hdisk".
   rewrite /jrnl_start /twophase_init.
-  destruct Hinit as (sz&kinds&Hsize2&Hnn&Heqi&Heqs&Hdom&Hkind_size).
+  destruct Hinit as (sz&kinds&Hsize2&Hnn&Hnonneg&Heqi&Heqs&Hdom&Hkind_size).
   rewrite Heqs Heqi.
   iIntros "(Hclosed_frag&Hjrnl_frag)".
   iDestruct "Hjrnl_frag" as "(Hsmapstos&Hcrashtoks&Hcrash_ctx&Hkinds&Hdom&Hfull)".
@@ -97,7 +97,7 @@ Qed.
 
 Lemma jrnl_init_obligation2: sty_init_obligation2 (twophase_initP JRNL_KIND_SIZE).
 Proof.
-  intros ???? (sz&?&Hsize2&?&?&?&Hdom&Hksz). rewrite //=. split_and!; eauto.
+  intros ???? (sz&?&Hsize2&?&?&?&?&Hdom&Hksz). rewrite //=. split_and!; eauto.
   eexists; split; eauto. eapply wf_jrnl_alt, kind_heap0_ok.
   { intros a Hin. revert Hin. rewrite Hdom elem_of_list_to_set elem_of_list_fmap; intros (?&->&Hin).
     apply elem_of_seqZ in Hin. clear -Hsize2 Hin. rewrite /block_bytes in Hsize2.
